Adjustments to typed_mapsto, eliminate the trailing unit

progs/list_dt.v
@@ -11,44 +11,45 @@ Import SequentialClight.SeqC.CSL.
 
 Local Open Scope logic.
 
-Class listspec (list_structid: ident) (list_link: ident) :=
+Class listspec (list_struct: type) (list_link: ident) :=
   mk_listspec {  
    list_fields: fieldlist;
-   list_struct: type := (Tstruct list_structid list_fields noattr);
+   list_structid: ident;
+   list_struct_eq: list_struct= Tstruct list_structid list_fields noattr;
    list_link_type: (type_of_field
           (unroll_composite_fields list_structid list_struct list_fields)
           list_link) = tptr list_struct
 }.
 
 Section LIST.
-Context  {list_structid} {list_link} (ls: listspec list_structid list_link).
+Context  {list_struct: type} {list_link: ident}.
 
-Definition list_cell sh p v :=
+Definition list_cell (ls: listspec list_struct list_link) sh p v :=
    field_mapsto_ sh list_struct list_link p -* typed_mapsto list_struct sh 0 p v.
 
-Definition lseg' (sh: share) := 
+Definition lseg' (ls: listspec list_struct list_link) (sh: share) := 
   HORec (fun (R: (list (reptype list_struct))*(val*val) -> mpred) (lp: (list (reptype list_struct))*(val*val)) =>
         match lp with
         | (h::hs, (first,last)) =>
                 (!! (~ (ptr_eq first last)) && 
                         EX tail:val, 
-                           list_cell sh first h
+                           list_cell ls sh first h
                            * field_mapsto sh list_struct list_link first tail
                            * |> R (hs, (tail, last)))
         | (nil, (first,last)) =>
                  !! (ptr_eq first last) && emp
         end).
 
-Definition lseg  (sh: share) (contents: list (reptype list_struct)) (x y: val) : mpred :=
-   lseg' sh (contents, (x,y)).
+Definition lseg (ls: listspec list_struct list_link) (sh: share) (contents: list (reptype list_struct)) (x y: val) : mpred :=
+   lseg' ls sh (contents, (x,y)).
 
-Lemma lseg_unfold: forall sh contents v1 v2,
-    lseg sh contents v1 v2 = 
+Lemma lseg_unfold (ls: listspec list_struct list_link): forall sh contents v1 v2,
+    lseg ls sh contents v1 v2 = 
      match contents with
      | h::t => !! (~ ptr_eq v1 v2) && EX tail: val,
-                      list_cell sh v1 h
+                      list_cell ls sh v1 h
                       * field_mapsto sh list_struct list_link v1 tail
-                      * |> lseg sh t tail v2
+                      * |> lseg ls sh t tail v2
      | nil => !! (ptr_eq v1 v2) && emp
      end.
 Proof.
@@ -62,13 +63,13 @@ Proof.
  auto 50 with contractive.
 Qed.
 
-Lemma lseg_eq:
+Lemma lseg_eq (ls: listspec list_struct list_link):
   forall sh l v , 
   typecheck_val v (tptr list_struct) = true ->
-    lseg sh l v v = !!(l=nil) && emp.
+    lseg ls sh l v v = !!(l=nil) && emp.
 Proof.
 intros.
-rewrite (lseg_unfold sh l v v).
+rewrite (lseg_unfold ls sh l v v).
 destruct l.
 f_equal. f_equal.
 apply prop_ext; split; intro; auto.
@@ -94,19 +95,19 @@ Qed.
 
 
 
-Definition lseg_cons sh (l: list (reptype list_struct)) (x z: val) : mpred :=
+Definition lseg_cons (ls: listspec list_struct list_link) sh (l: list (reptype list_struct)) (x z: val) : mpred :=
         !! (~ ptr_eq x z) && 
        EX h:(reptype list_struct), EX r:list (reptype list_struct), EX y:val, 
              !!(l=h::r  /\ typecheck_val y (tptr list_struct) = true) && 
-             list_cell sh x h *
+             list_cell ls sh x h *
              field_mapsto sh list_struct list_link x y * 
-             |> lseg sh r y z.
+             |> lseg ls sh r y z.
 
-Lemma lseg_neq:  forall sh l x z , 
+Lemma lseg_neq (ls: listspec list_struct list_link):  forall sh l x z , 
   typecheck_val x (tptr list_struct) = true ->
   typecheck_val z (tptr list_struct) = true ->
   ptr_neq x z -> 
-    lseg sh l x z = lseg_cons sh l x z.
+    lseg ls sh l x z = lseg_cons ls sh l x z.
 Proof.
 unfold lseg_cons, ptr_neq; intros.
 rewrite lseg_unfold at 1; auto.
@@ -126,7 +127,8 @@ apply exp_right with r.
 apply exp_right with l.
 apply exp_right with tail.
 repeat rewrite sepcon_andp_prop'; apply andp_right.
-rewrite (field_mapsto_typecheck_val list_struct list_link sh x tail list_structid list_fields noattr) by auto.
+rewrite (field_mapsto_typecheck_val list_struct list_link sh x tail list_structid list_fields noattr)
+  by apply list_struct_eq.
 rewrite list_link_type.
 normalize. auto.
 apply exp_left; intro h.
@@ -140,8 +142,8 @@ apply exp_right with y.
  auto.
 Qed.
 
-Lemma lseg_unroll: forall sh l x z , 
-    lseg sh l x z = (!! (ptr_eq x z) && !! (l=nil) && emp) || lseg_cons sh l x z.
+Lemma lseg_unroll (ls: listspec list_struct list_link): forall sh l x z , 
+    lseg ls sh l x z = (!! (ptr_eq x z) && !! (l=nil) && emp) || lseg_cons ls sh l x z.
 Proof.
 intros.
 rewrite lseg_unfold at 1.
@@ -161,6 +163,7 @@ apply andp_right.
 erewrite (field_mapsto_typecheck_val list_struct list_link sh x tail); try reflexivity.
 rewrite list_link_type.
 normalize.
+apply list_struct_eq.
 auto.
 apply orp_left; normalize.
 unfold lseg_cons.
@@ -185,14 +188,14 @@ right; intros [? ?]. contradiction.
 Qed.
 
 
-Lemma lseg_unroll_nonempty1:
+Lemma lseg_unroll_nonempty1 (ls: listspec list_struct list_link):
    forall p P sh h tail v1 v2,
     ~ ptr_eq v1 v2 ->
     typecheck_val p (tptr list_struct) = true ->
-    P |-- list_cell sh v1 h *
+    P |-- list_cell ls sh v1 h *
              (field_mapsto sh list_struct list_link v1 p *
-               lseg sh tail p v2) ->
-    P |-- lseg sh (h::tail) v1 v2.
+               lseg ls sh tail p v2) ->
+    P |-- lseg ls sh (h::tail) v1 v2.
 Proof. intros. rewrite lseg_unroll. apply orp_right2. unfold lseg_cons.
   rewrite prop_true_andp by auto.
   apply exp_right with h. apply exp_right with tail. apply exp_right with p.
@@ -204,10 +207,10 @@ Proof. intros. rewrite lseg_unroll. apply orp_right2. unfold lseg_cons.
  apply now_later.
 Qed.
 
-Lemma lseg_nonnull:
+Lemma lseg_nonnull (ls: listspec list_struct list_link):
   forall sh s v,
       typed_true (tptr list_struct) v ->
-     lseg sh s v nullval = lseg_cons sh s v nullval.
+     lseg ls sh s v nullval = lseg_cons ls sh s v nullval.
 Proof.
 intros. subst. 
 rewrite lseg_unroll.
@@ -219,15 +222,15 @@ rewrite H0 in H. inv H.
 apply orp_right2. auto.
 Qed.
 
-Lemma lift2_lseg_cons: 
- forall sh s p q, `(lseg_cons sh s)  p q =
+Lemma lift2_lseg_cons (ls: listspec list_struct list_link): 
+ forall sh s p q, `(lseg_cons ls sh s)  p q =
     EX hry:(reptype list_struct * list (reptype list_struct) * val),
       match hry with (h,r,y) =>
        !! (s = h::r) &&
        (local (`ptr_neq p q) &&
-       (`(list_cell sh) p (`h) *
+       (`(list_cell ls sh) p (`h) *
         `(field_mapsto sh list_struct list_link) p (`y) *
-        |> `(lseg sh r) (`y) q))
+        |> `(lseg ls sh r) (`y) q))
      end.
 Proof.
  intros.
@@ -239,32 +242,32 @@ Proof.
  apply exp_right with r.
  apply exp_right with y. normalize.
  apply andp_right.
- erewrite (field_mapsto_typecheck_val); [ | reflexivity].
+ erewrite (field_mapsto_typecheck_val); [ | apply list_struct_eq].
  rewrite list_link_type. normalize. auto.
 Qed.
 
-Lemma unfold_lseg_cons:
+Lemma unfold_lseg_cons (ls: listspec list_struct list_link):
    forall P Q1 Q R e sh s,
       local Q1 &&
-      PROPx P (LOCALx Q (SEPx (`(lseg sh s) e (`nullval) :: R))) |-- 
+      PROPx P (LOCALx Q (SEPx (`(lseg ls sh s) e (`nullval) :: R))) |-- 
                         local (`(typed_true (tptr list_struct)) e) ->
-      local Q1 && PROPx P (LOCALx Q (SEPx (`(lseg sh s) e (`nullval) :: R))) |--
+      local Q1 && PROPx P (LOCALx Q (SEPx (`(lseg ls sh s) e (`nullval) :: R))) |--
      EX hry: reptype list_struct * list (reptype list_struct) * val,
       match hry with (h,r,y) => 
        !! (s=h::r) &&
       PROPx P (LOCALx Q 
-        (SEPx (`(list_cell sh) e (`h) ::
+        (SEPx (`(list_cell ls sh) e (`h) ::
                   `(field_mapsto sh list_struct list_link) e (`y) ::
-                  |> `(lseg sh r) (`y) (`nullval) ::
+                  |> `(lseg ls sh r) (`y) (`nullval) ::
                   R)))
         end.
 Proof.
 intros.
 apply derives_trans with
-(local Q1 && PROPx P (LOCALx Q (SEPx (`(lseg_cons sh s) e (`nullval) :: R)))).
+(local Q1 && PROPx P (LOCALx Q (SEPx (`(lseg_cons ls sh s) e (`nullval) :: R)))).
 apply derives_trans with
 (local Q1 && local (`(typed_true (tptr list_struct)) e) &&
- PROPx P (LOCALx Q (SEPx (`(lseg sh s) e (`nullval) :: R)))).
+ PROPx P (LOCALx Q (SEPx (`(lseg ls sh s) e (`nullval) :: R)))).
 apply andp_right; auto.
 apply andp_right; auto.
 apply andp_left1; auto.
@@ -287,19 +290,19 @@ normalize.
  auto.
 Qed.
 
-Lemma semax_lseg_nonnull:
+Lemma semax_lseg_nonnull (ls: listspec list_struct list_link):
   forall Delta P Q sh s e R c Post,
    PROPx P (LOCALx (tc_environ Delta :: Q)
-            (SEPx (`(lseg sh s) e (`nullval) :: R))) |-- 
+            (SEPx (`(lseg ls sh s) e (`nullval) :: R))) |-- 
                         local (`(typed_true (tptr list_struct)) e)  ->
   (forall (h: reptype list_struct) (r: list (reptype list_struct)) (y: val), s=h::r ->
     semax Delta 
         (PROPx P (LOCALx Q 
-        (SEPx (`(list_cell sh) e (`h) ::
+        (SEPx (`(list_cell ls sh) e (`h) ::
                   `(field_mapsto sh list_struct list_link) e (`y) ::
-                  |> `(lseg sh r) (`y) (`nullval) ::
+                  |> `(lseg ls sh r) (`y) (`nullval) ::
                   R)))) c Post) ->
-  semax Delta (PROPx P (LOCALx Q (SEPx (`(lseg sh s) e (`nullval) :: R)))) c Post.
+  semax Delta (PROPx P (LOCALx Q (SEPx (`(lseg ls sh s) e (`nullval) :: R)))) c Post.
 Proof.
 intros.
 eapply semax_pre;  [apply unfold_lseg_cons | ].
@@ -309,8 +312,8 @@ apply extract_exists_pre; intros [[h r] y].
 apply semax_extract_prop; intro; auto.
 Qed.
 
-Lemma lseg_nil_eq: 
-    forall sh p q, lseg sh nil p q = !! (ptr_eq p q) && emp.
+Lemma lseg_nil_eq (ls: listspec list_struct list_link): 
+    forall sh p q, lseg ls sh nil p q = !! (ptr_eq p q) && emp.
 Proof. intros.
  rewrite lseg_unroll.
  apply pred_ext.
@@ -319,14 +322,14 @@ Proof. intros.
  apply orp_right1. normalize.
 Qed.
 
-Lemma lseg_cons_eq:
+Lemma lseg_cons_eq (ls: listspec list_struct list_link):
      forall sh h r x z , 
-    lseg sh (h::r) x z = 
+    lseg ls sh (h::r) x z = 
         !!(~ ptr_eq x z) &&
          (EX  y : val,
           !!(typecheck_val y (tptr list_struct) = true) &&
-   list_cell sh x h * field_mapsto sh list_struct list_link x y *
-   |>lseg sh r y z).
+   list_cell ls sh x h * field_mapsto sh list_struct list_link x y *
+   |>lseg ls sh r y z).
 Proof.
  intros. rewrite lseg_unroll.
  apply pred_ext.
@@ -352,17 +355,17 @@ Proof.
  apply prop_derives; intuition.
 Qed.
 
-Definition lseg_cons_right sh (l: list (reptype list_struct)) (x z: val) : mpred :=
+Definition lseg_cons_right (ls: listspec list_struct list_link) sh (l: list (reptype list_struct)) (x z: val) : mpred :=
         !! (~ ptr_eq x z) && 
        EX h:(reptype list_struct), EX r:list (reptype list_struct), EX y:val, 
              !!(l=r++h::nil)  && 
-                       list_cell sh y h *
+                       list_cell ls sh y h *
              field_mapsto sh list_struct list_link y z * 
-             |> lseg sh r x y.
+             |> lseg ls sh r x y.
 
 
-Lemma lseg_unroll_right: forall sh l x z , 
-    lseg sh l x z = (!! (ptr_eq x z) && !! (l=nil) && emp) || lseg_cons_right sh l x z.
+Lemma lseg_unroll_right (ls: listspec list_struct list_link): forall sh l x z , 
+    lseg ls sh l x z = (!! (ptr_eq x z) && !! (l=nil) && emp) || lseg_cons_right ls sh l x z.
 Admitted.
 
 End LIST.
@@ -370,6 +373,3 @@ End LIST.
 Hint Rewrite @lseg_nil_eq : normalize.
 
 Hint Rewrite @lseg_eq using reflexivity: normalize.
-
-
-
